Add: fix tableau definition and prove soundness for propositional fragment

theories/Proofs.v
@@ -4,6 +4,63 @@ From Tableaux Require Import Semantics.
 From Tableaux Require Import Skolemization.
 From Tableaux Require Import Syntax.
 
+(** ** Contexts *)
+
+(** As we want to keep a [sko_record] in the contexts, contexts get parameterized by
+    skolemization instances. *)
+Section Contexts.
+  Context `{set_nat : set nat} {pred func var : Atom} {sko : Skolemization_ pred func var}.
+
+  Record Con_ :=
+    { forms : list (Form_ pred func var)
+    ; con_sko_record : sko_record sko }.
+
+  Definition empty_ctx : Con_ :=
+    {| forms := []
+    ;  con_sko_record := empty_record |}.
+
+  Definition in_ctx (F : Form_ pred func var) (Gamma : Con_) : Prop :=
+    List.In F (forms Gamma).
+
+  Definition extend_ctx (Gamma : Con_) (A : Form_ pred func var) : Con_ :=
+    {| forms := A :: forms Gamma
+    ;  con_sko_record := con_sko_record Gamma |}.
+
+  Fixpoint fv_ctx_ (Gamma : list (Form_ pred func var)) : set_atom var :=
+    match Gamma with
+    | [] => empty_set
+    | F :: Fs => fv F \union fv_ctx_ Fs
+    end.
+
+  #[global] Instance fv_ctx : @FV var Con_ :=
+    fun Gamma => fv_ctx_ (forms Gamma).
+
+  Fixpoint subst_ctx_ (Gamma : list (Form_ pred func var)) (sigma : Substitution var (Term_ func var))
+    : list (Form_ pred func var) :=
+    match Gamma with
+    | [] => []
+    | F :: Fs => F@[sigma] :: subst_ctx_ Fs sigma
+    end.
+
+  #[global] Instance subst_ctx : Subst Con_ (Term_ func var) :=
+    fun Gamma sigma =>
+      {| forms := subst_ctx_ (forms Gamma) sigma
+      ;  con_sko_record := con_sko_record Gamma |}. (* TODO: we probably want to subst this *)
+
+  Definition set_con_sko_record (record : sko_record sko) (Gamma : Con_) : Con_ :=
+    {| forms := forms Gamma
+    ;  con_sko_record := record |}.
+End Contexts.
+
+Arguments Con_ : clear implicits.
+
+Notation "Gamma ,, A" := (extend_ctx Gamma A) (at level 20).
+Notation "A \in Gamma" := (in_ctx A Gamma) (at level 30).
+Notation "{{ }}" := (empty_ctx).
+Notation "{{ F }}" := (empty_ctx ,, F).
+Notation "{{ F1 ;; F2 ;; .. ;; Fk }}" :=
+  (extend_ctx .. (extend_ctx (extend_ctx empty_ctx F1) F2) .. Fk).
+
 Section TableauxProofs.
   Context `{set_nat : set nat} {pred func var : Atom} (sko : Skolemization_ pred func var).
 
@@ -11,7 +68,7 @@ Section TableauxProofs.
 
   Let set_var := set_atom var.
   Let set_func := set_atom func.
-  Let Con := Con_ pred func var.
+  Let Con := Con_ pred func var sko.
   Let Term := Term_ func var.
   Let Form := Form_ pred func var.
   Let sko_record := sko_record sko.
@@ -47,14 +104,16 @@ Section TableauxProofs.
   | hasTableauAll :
     forall (Gamma : Con) (S : set_var) (Sf : sko_record) (sigma : Substitution var Term)
       (x : var) (F : Form),
-      (All F) \in Gamma -> isFresh x S -> hasTableau_ (Gamma ,, F{0 \to Free x}) S Sf sigma ->
+      (All F) \in Gamma -> isFresh x (fv Gamma) -> hasTableau_ (Gamma ,, F{0 \to Free x}) S Sf sigma ->
       hasTableau_ Gamma (add x S) Sf sigma
 
    (** Delta rule *)
   | hasTableauNegAll :
     forall (Gamma : Con) (S : set_var) (Sf : sko_record) (sigma : Substitution var Term)
-      (F : Form) (t : Term) (Hsko : is_sko t (Neg F) (fv Gamma) Sf),
-      (Neg (All F)) \in Gamma -> hasTableau_ (Gamma ,, Neg F{0 \to t}) S Sf sigma ->
+      (F : Form) (t : Term) (Hsko : is_sko t (Neg F) (fv Gamma) (con_sko_record Gamma)),
+      (Neg (All F)) \in Gamma -> hasTableau_ (set_con_sko_record
+                                       (add_symbol (symbol sko t Hsko) F (con_sko_record Gamma))
+                                       (Gamma ,, Neg F{0 \to t})) S Sf sigma ->
       hasTableau_ Gamma S (add_symbol (symbol sko t Hsko) F Sf) sigma.
 
   Definition hasTableau (Gamma : Con) (sigma : Substitution var Term) : Prop :=
@@ -66,16 +125,64 @@ End TableauxProofs.
 Section TableauxSoundness.
   Context `{set_nat : set nat} {pred func var : Atom} (sko : Skolemization_ pred func var).
 
-  Theorem hasTableau_sound :
-    forall (F : Form_ pred func var) (sigma : Substitution var (Term_ func var)),
-      hasTableau sko {{ Neg F }} sigma -> \models F.
-  Proof.
-    Admitted.
+  Let Con := Con_ pred func var sko.
+  Let Form := Form_ pred func var.
+  Let Term := Term_ func var.
 
-(* Theorem hasTableau_sound : *)
-(*     forall (Gamma : Con_ pred func var) (sigma : Substitution var (Term_ func var)), *)
-(*       hasTableau sko Gamma sigma -> is_countersat (con_to_formula Gamma). *)
-(*   Proof. *)
-(*     intros ?? (S & Sf & htab). induction htab. *)
-(*     Admitted. *)
+  Lemma subst_ctx_subst_list :
+    forall (Gamma : Con) (sigma : Substitution var Term),
+      (forms Gamma)@[sigma] = forms (Gamma@[sigma]).
+  Proof using Type.
+    intros [l sko_] sigma; cbn. clear sko_; induction l as [|F Fs IHFs]; auto.
+    cbn. f_equal. apply IHFs.
+  Qed.
+
+  Lemma in_ctx_in_substituted_ctx :
+    forall (Gamma : Con) (F : Form) (sigma : Substitution var Term),
+      F \in Gamma -> F@[sigma] \in Gamma@[sigma].
+  Proof using Type.
+    intros ???. destruct Gamma as [l sko_]; cbn. clear sko_.
+    induction l as [|G Gs IHGs]; intros Hin; inversion Hin.
+    - rewrite H. cbn. now left.
+    - right. now apply IHGs.
+  Qed.
+
+  Theorem hasTableau_sound :
+    forall (sigma : Substitution var Term) (Gamma : Con) (F : Form),
+      hasTableau sko (Gamma ,, Neg F) sigma -> ((forms Gamma)@[sigma] \models F@[sigma]).
+  Proof.
+    intros ??? (S & Sf & htab).
+    rewrite models_iff. replace (Neg F@[sigma] :: (forms Gamma)@[sigma]) with (forms (Gamma ,, Neg F)@[sigma]).
+    2: { rewrite subst_ctx_subst_list. now cbn. }
+    induction htab.
+    - apply in_form_list_models.
+      apply in_ctx_in_substituted_ctx with (sigma := sigma) in H.
+      now cbn in H.
+    - apply in_ctx_in_substituted_ctx with (sigma := sigma) in H0, H.
+      apply models_P_neg_P with (F := P@[sigma]).
+      + now apply in_form_list_models.
+      + apply in_form_list_models. now rewrite H1.
+    - apply extend_with_equiv_form with (F := F0@[sigma]) (G := Neg (Neg F0@[sigma])); auto.
+      + apply neg_neg_equiv.
+      + now apply in_ctx_in_substituted_ctx with (sigma := sigma) in H.
+    - apply extend_with_double_equiv_form with (F1 := Neg F2@[sigma]) (F2 := Neg F1@[sigma])
+                                               (G := Neg (Or F1 F2)@[sigma]); auto.
+      + apply neg_equiv. cbn.
+        rewrite or_comm. apply or_equiv.
+        all: symmetry; apply neg_neg_equiv.
+      + now apply in_ctx_in_substituted_ctx with (sigma := sigma) in H.
+    - apply double_extend_with_equiv_form with (F1 := F1@[sigma]) (F2 := F2@[sigma]) (G := (Or F1 F2)@[sigma]);
+        auto.
+      + reflexivity.
+      + now apply in_ctx_in_substituted_ctx with (sigma := sigma) in H.
+    - apply extend_with_equiv_form with (F := F0 {0 \to Free x}@[sigma]) (G := (All F0)@[sigma]); auto.
+      + admit.
+      + now apply in_ctx_in_substituted_ctx with (sigma := sigma) in H.
+  Admitted.
 End TableauxSoundness.
+
+Module ConcreteProofInstances.
+  Export ConcreteSkolemizationInstances.
+
+  Definition Con := Con_ string string string.
+End ConcreteProofInstances.
