theories/Syntax.v
@@ -228,57 +228,6 @@ Section FVForms.
       end.
 End FVForms.
 
-(** ** Contexts *)
-Section Contexts.
-  Context {pred func var : Atom}.
-
-  Record Con_ :=
-    { forms : list (Form_ pred func var)
-    ; sko_symbols_form : list (func * Form_ pred func var) }.
-
-  Definition empty_ctx : Con_ :=
-    {| forms := []
-    ;  sko_symbols_form := [] |}.
-
-  Definition in_ctx (F : Form_ pred func var) (Gamma : Con_) : Prop :=
-    List.In F (forms Gamma).
-
-  Definition extend_ctx (Gamma : Con_) (A : Form_ pred func var) : Con_ :=
-    {| forms := A :: forms Gamma
-    ;  sko_symbols_form := sko_symbols_form Gamma |}.
-
-  Fixpoint fv_ctx_ (Gamma : list (Form_ pred func var)) : set_atom var :=
-    match Gamma with
-    | [] => empty_set
-    | F :: Fs => fv F \union fv_ctx_ Fs
-    end.
-
-  Definition fv_ctx : @FV var Con_ :=
-    fun Gamma => fv_ctx_ (forms Gamma).
-
-  Fixpoint skolem_symbols_ctx_ (l : list (func * Form_ pred func var)) : set_atom func :=
-    match l with
-    | [] => empty_set
-    | (f , _) :: xs => add f (skolem_symbols_ctx_ xs)
-    end.
-
-  Definition skolem_symbols_ctx (Gamma : Con_) : set_atom func :=
-    skolem_symbols_ctx_ (sko_symbols_form Gamma).
-
-  Definition add_skolem_symbol_ctx (f : func) (F : Form_ pred func var) (Gamma : Con_) : Con_ :=
-    {| forms := forms Gamma
-    ;  sko_symbols_form := (f, F) :: sko_symbols_form Gamma |}.
-End Contexts.
-
-Arguments Con_ : clear implicits.
-
-Notation "Gamma ,, A" := (extend_ctx Gamma A) (at level 20).
-Notation "A \in Gamma" := (in_ctx A Gamma) (at level 30).
-Notation "{{ }}" := (empty_ctx).
-Notation "{{ F }}" := (empty_ctx ,, F).
-Notation "{{ F1 ;; F2 ;; .. ;; Fk }}" :=
-  (extend_ctx .. (extend_ctx (extend_ctx empty_ctx F1) F2) .. Fk).
-
 (** ** Utils functions *)
 Definition get_symbol {func var : Atom} (t : Term_ func var) : option func :=
   match t with
@@ -292,7 +241,6 @@ Module ConcreteSyntaxInstances.
 
   Definition Term := Term_ string string.
   Definition Form := Form_ string string string.
-  Definition Con := Con_ string string string.
 
   (** *** Set of [Term]s. *)
   Module OrderedTerm <: SimpleOrderedType.
