theories/Prelude/Init.v
@@ -9,3 +9,8 @@ Export ListNotations.
 Open Scope string_scope.
 
 Notation "#| l |" := (List.length l).
+
+Axiom prodext :
+  forall {A : Type} {P Q : A -> Prop},
+    (forall x : A, P x = Q x) ->
+    (forall x : A, P x) = (forall x : A, Q x).
